\documentclass{article}
\usepackage[utf8]{inputenc}
\usepackage{setspace}
\usepackage{tikz}
\usetikzlibrary{positioning}
\usepackage{amsfonts}
\usepackage{amssymb}
\usepackage{amsmath}
\usepackage{amsthm}
\usepackage{systeme}
\usepackage{mathtools}
\usepackage{hyperref}
\usepackage{venndiagram}
\usepackage{pgfplots}
\usetikzlibrary{pgfplots.statistics}
\pgfplotsset{compat=newest}

\begin{document}

\section*{Question 1}

~

\subsection*{a}

~

\begin{align*}
    &E[Y|X=x]=\int_{0}^{x}yf_{Y|X}(y|x)dy\\
    &=\int_{0}^{x}y\frac{1}{x}dy\\
    &=\frac{y^2}{2}\frac{1}{x}|_{0}^{x}\\
    &=\frac{x}{2}\\
    \Rightarrow&E[Y|X=x]\text{ is a linear function of }x\\
    &E[Y^2|X=x]=\int_{0}^{x}y^2f_{Y|X}(y|x)dy\\
    &=\left[\frac{y^3}{3}\frac{1}{x}\right]_{0}^{x}\\
    &=\frac{x^2}{3}\\
    &V[Y|X=x]=E[Y^2|X=x]-(E[Y|X=x])^2=\frac{x^2}{3}-frac{x^2}{4}=\frac{x^2}{12}\\
\end{align*}

~

\subsection*{b}

~

\begin{align*}
    &f(x,y)=f_{Y|X}(y|x)f_X(x)=\frac{1}{x}\times 1=\frac{1}{x}\\
\end{align*}

~

\subsection*{c}

~

\begin{align*}
    &0\leqslant y\leqslant x\leqslant 1\\
    \Rightarrow&f_Y(y)=\int_{y}^{1}f(x,y)dx\\
    &=\int_{y}^{1}\frac{1}{x}dx\\
    &=\left[\ln (x)\right]^{1}_{y}\\
    &=-\ln (y),y\in[0,1]\\
\end{align*}

~

\subsection*{d}

~

\begin{align*}
    &E[Y]=\int_{0}^{1}yf_Y(y)dy\\
    &=\int_{0}^{1}y(-\ln(y))dy\\
    &=\left[-\ln (y)\int ydy+\int(\frac{d}{dy}\ln(y)\int ydy )dy\right]^{1}_{0}\\
    &=\left[-\frac{x^2}{2}\ln(y)+\frac{y^2}{4}\right]^{1}_{0}\\
    &=\frac{1}{4}\\
\end{align*}

\newpage

\section*{Question 2}

~

\subsection*{a}

~

\begin{align*}
    &f(x,y)=2e^{-(x+y)}\\
    &f_X(x)=\int_{x}^{+\infty}f(x,y)dy\\
    &=\int_{x}^{+\infty}2e^{-(x+y)}dy\\
    &=\left[-2e^{-(x+y)}\right]^{+\infty}_{x}\\
    &=2e^{-2x},x>0\\
\end{align*}

~

\subsection*{b}

~

\begin{align*}
    &f_{Y|X}(y|x)=\frac{f(x,y)}{f_X(x)}\\
    &=\frac{2e^{-(x+y)}}{2e^{-2x}}=e^{x-y},x<y\\
\end{align*}

~

\subsection*{c}

~

\begin{align*}
    &f_{Y|X}(y|x=1)=e^{1-y},y>1\\
    &P(y>2|x=1)=\int_{2}^{+\infty}f_{Y|X}(y|x=1)dy\\
    &=\int_{2}^{+\infty}e^{1-y}dy\\
    &=\left[-e^{1-y}\right]^{+\infty}_{2}\\
    &=e^{-1}\\
\end{align*}

~

\subsection*{d}

~

\begin{align*}
    &f_Y(y)=\int_{0}^{y}f(x,y)dx\\
    &=\int_{0}^{y}2e^{-(x+y)}dx\\
    &=\left[-2e^{-(x+y)}\right]_{0}^{y}\\
    &=2e^{-y}-2e^{-2y}\\
    &f_X(x)f_Y(y)=2e^{-2x}(2e^{-y}-2e^{-2y})\ne 2e^{-(x+y)}\\
    \Rightarrow&f_X(x)f_Y(y)\ne f(x,y)\implies \text{dependent}\\
\end{align*}

~

\subsection*{e}

~

\begin{align*}
    &E[Y|X=x]=\int_{x}^{+\infty}yf_{Y|X}(y|x)dy\\
    &=\int_{x}^{+\infty}ye^{x-y}dy\\
    &=\left[ y \int e^{x-y}dy-\int(\frac{d}{dy}y\int e^{x-y}dy)dy\right]^{+\infty}_{x}\\
    &=\left[-ye^{x-y}-e^{x-y}\right]^{+\infty}_{x}\\
    &=x+1\\
    \Rightarrow&\text{it is linear}\\
\end{align*}

~

\subsection*{f}

~

\begin{align*}
    &f_{Y|X}(y|x)=e^{x-y}\\
    &E[Y^2|X=x]=\int_{x}^{\infty}y^2f_{Y|X}(y|x)dy\\
    &=\int_{x}^{\infty}y^2e^{x-y}dy\\
    &=\left[y^2\int e^{x-y}dy-\int(\frac{d}{dy}y^2\int e^{x-y}dy)dy\right]_{x}^{+\infty}\\
    &=\left[-y^2e^{x-y}+2\int ye^{x-y}dy\right]_{x}^{+\infty}\\
    &=\left[-y^2e^{x-y}+2(-ye^{x-y}-e^{x-y})\right]_{x}^{+\infty}\\
    &=x^2+2x+2\\
    &V[Y|X=x]=E[Y^2|X=x]-(E[Y|X=x])^2\\
    &=x^2+2x+2-(x+1)^2\\
    &=1\\
\end{align*}

\newpage

\section*{Question 3}

~

\subsection*{a}

~

\begin{tikzpicture}
    \begin{axis}[axis lines=left,]
       \addplot[
            domain=0:1,
            samples =100,
            color=black,
       ]
        {3*(1-x)^2};
        \addplot[
            domain=1:2,
            samples =100,
            color=black,
        ]
        {0};
    \end{axis}
\end{tikzpicture}

~

\subsection*{b}

~

\begin{tikzpicture}
    \begin{axis}[axis lines=left,]
        \addplot[
            domain=0:1,
            samples =100,
            color=black,
        ]
        {(1-x)^3};
    \end{axis}
\end{tikzpicture}

~

\subsection*{c}

~

\begin{align*}
    &Y=(1-X)^3\\
    \Rightarrow&X=1-Y^{\frac{1}{3}}\\
    &\frac{dx}{dy}=-\frac{1}{3}y^{-\frac{2}{3}}\\
    &f_Y(y)=f_X(x)\left|\frac{dx}{dy}\right|\\
    &=3(1-(1-y^{\frac{1}{3}}))^2\frac{1}{3}y^{-frac{2}{3}}\\
    &=1\\
\end{align*}

\newpage

\section*{Question 4}

~

\subsection*{d}

~


\begin{tikzpicture}
    \begin{axis}[axis lines=left,]
       \addplot[
            domain=0:1,
            samples =100,
            color=black,
       ]
        {3*x^2};
        \addplot[
            domain=1:2,
            samples =100,
            color=black,
        ]
        {0};
    \end{axis}
\end{tikzpicture}

~

\subsection*{e}

~

\begin{tikzpicture}
    \begin{axis}[axis lines=left,]
        \addplot[
            domain=0:1,
            samples =100,
            color=black,
        ]
        {x^2};
    \end{axis}
\end{tikzpicture}

~

\subsection*{f}

~

\begin{align*}
    &y=x^2,x,y\in[0,1]\\
    &x=\sqrt{y},x,y\in[0,1]\\
    \Rightarrow&g_Y(y)=\sqrt{y}\\
\end{align*}

~

\subsection*{g}

~

\begin{align*}
    &{g_Y}'(y)=\frac{1}{2\sqrt{y}},y\in[0,1]\\
\end{align*}

~

\subsection*{h}

~

\begin{align*}
    &f_Y(y)=f_X(x)\left|\frac{dx}{dy}\right|\\
    &=3(\sqrt{y})^2\frac{1}{2\sqrt{y}}\\
    &=\frac{3}{2}\sqrt{y},y\in[0,1]\\
\end{align*}

\newpage

\section*{Question 5}

~

\subsection*{a}

~

\begin{align*}
    &P(X=1,Y=1)=0.030\\
\end{align*}

~

\subsection*{b}

~

\begin{align*}
    &P(X\leqslant 1,Y\leqslant 1)\\
    &=P(X=0,Y=0)+P(X=0,Y=1)\\
    &+P(X=1,Y=0)+P(X=1,Y=1)\\
    &=0.025+0.015+0.050+0.030=0.120\\
\end{align*}

~

\subsection*{c}

~

\begin{align*}
    &P(X=1)=P(X=1,Y=0)+P(X=1,Y=1)+P(X=1,Y=2)\\
    &=0.050+0.030+0.020=0.100\\
    &P(Y=1)=P(X=0,Y=1)+P(X=1,Y=1)+P(X=2,Y=1)\\
    &+P(X=3,Y=1)+P(X=4,Y=1)+P(X=5,Y=1)\\
    &=0.015+0.030+0.075+0.090+0.060+0.030\\
    &=0.300\\
\end{align*}

~

\subsection*{d}

~

\begin{align*}
    &X+3Y>5\\
    &Y=0: \text{no overflow}\\
    &Y=1:X=3,4,5\\
    &P(X\leqslant 3,Y=1)=0.090+0.060+0.030=0.18\\
    &Y=2:X=1,2,3,4,5\\
    &P(Y=2)=0.010+0.020+0.050+0.060+0.040+0.020\\
    &=0.200\\
    \Rightarrow&P(X+3Y>5)=P(X\leqslant 3,Y=1)+P(Y=2)=0.180+0.200=0.380\\
\end{align*}

~

\subsection*{e}

~

\begin{align*}
    &\forall x\in[0,5],y\in[0,2],P(X=x,Y=y)=P(X=x)P(Y=y)\\
    \Rightarrow&\text{Independent}\\
\end{align*}

\newpage

\section*{Question 6}

~

\begin{align*}
    &P(X=0)=0.025+0.015+0.010=0.050\\
    &P(X=1)=0.050+0.030+0.020=0.100\\
    &P(X=2)=0.125+0.075+0.050=0.250\\
    &P(X=3)=0.150+0.090+0.060=0.300\\
    &P(X=4)=0.100+0.060+0.040=0.200\\
    &P(X=5)=0.050+0.030+0.020=0.100\\
    &E[X]=0P(X=0)+1P(X=1)+2P(X=2)+3P(X=3)+4P(X=4)+5P(X=5)\\
    &=0\times0.05+1\times 0.1+2\times 0.25+3\times 0.3+4\times 0.2+5\times 0.1=2.8\\
    &P(Y=0)=0.025+0.050+0.125+0.150+0.100+0.050=0.500\\
    &P(Y=1)=0.015+0.030+0.075+0.090+0.060+0.030=0.300\\
    &P(Y=2)=0.010+0.020+0.050+0.060+0.040+0.020=0.200\\
    &E[Y]=0P(Y=0)+1P(Y=1)+2P(Y=2)\\
    &=0\times 0.5+1\times 0.3+2\times 0.2=0.7\\
    &E[3X+10Y]=3E[X]+10E[Y]=3\times 2.8+10\times 0.7=15.4\\
\end{align*}

\newpage

\section*{Question 7}

~

\begin{align*}
    &F_X(x)=3x^2,x\in[0,1]\\
    &F_Y(y)=2y,y\in[0,1]\\
    &\text{Independent}\implies F(x,y)=f_X(x)F_Y(y)=3x^22y=6x^2y,x,y\in[0,1]\\
    &E[\left|X-Y\right|]=\int_{0}^{1}\int_{0}^{x}(x-y)6x^2y dydx+\int_{0}^{1}\int_{x}^{1}(y-x)6x^2y dydx\\
    &\int_{0}^{1}\int_{0}^{x}(x-y)6x^2y dydx\\
    =&\int_{0}^{1}\int_{0}^{x}6x^3y-6x^2y^2dydx\\
    =&\int_{0}^{1}\left[ 3x^3y^2-2x^2y^3\right]^{x}_{0}\\
    =&\int_{0}^{1}x^5dx\\
    =&\left[\frac{1}{6}x^6\right]^{1}_{0}\\
    =&\frac{1}{6}\\
    &\int_{0}^{1}\int_{x}^{1}(y-x)6x^2y dydx\\
    =&\int_{0}^{1}\int_{x}^{1}6x^2y^2-6x^3ydydx\\
    =&\int_{0}^{1}\left[2x^2y^3-3x^3y^2\right]^{1}_{x}\\
    =&\int_{0}^{1}2x^2-3x^3+x^5dx\\
    =&\left[\frac{2}{3}x^3-\frac{3}{4}x^4+\frac{1}{6}x^6\right]_{0}^{1}\\
    =&\frac{1}{12}\\
    \Rightarrow&E[\left|X-Y\right|]=\int_{0}^{1}\int_{0}^{x}(x-y)6x^2y dydx+\int_{0}^{1}\int_{x}^{1}(y-x)6x^2y dydx\\
    =&\frac{1}{6}+\frac{1}{12}\\
    =&\frac{1}{4}\\
\end{align*}

\newpage

\section*{Collaborators}

~

Frank Zhu

~

Jeffery Shu

~

Sam Sun
\end{document}