\documentclass{article}
\usepackage[utf8]{inputenc}
\usepackage{setspace}
\usepackage{tikz}
\usetikzlibrary{positioning}
\usepackage{amsfonts}
\usepackage{amssymb}
\usepackage{amsmath}
\usepackage{amsthm}
\usepackage{systeme}
\usepackage{mathtools}
\usepackage{hyperref}
\usepackage{venndiagram}
\usepackage{pgfplots}
\usetikzlibrary{pgfplots.statistics}
\pgfplotsset{compat=newest}

\begin{document}
\section*{Question 1}

~

\begin{align*}
    &f(x)=\frac{1}{10-0}=\frac{1}{10}\\
    &F(Y)=\frac{y}{10}\\
\end{align*}

~

\subsection*{a}

~

\begin{align*}
    &F(Y_L)=F(Y_1)\times F(Y_2)\times F(Y_3)\times F(Y_4)\times F(Y_5)\\
    &=F(Y)^5\\
    &=(\frac{y}{10})^5\\
    &=\frac{y^5}{10^5}\\
    &f(Y_L)=\frac{d}{dy}F(y_L)=\frac{5y^4}{10^5}\\
    &E(Y_L)=\int_{0}^{10}yf(Y_L)dy\\
    &=\int_{0}^{10}\frac{5y^5}{10^5}\\
    &=\left[\frac{5y^6}{6\times10^5}\right]^{10}_{0}\\
    &=\frac{5\times10^6}{6\times10^5}\\
    &=8.33\\
\end{align*}

~

\subsection*{b}

~

\begin{align*}
    &G(Y_S)=P(Y_1\leqslant Y)\\
    &=1-P(Y_1>Y)\\
    &=1-P[X_1>Y,X_2>Y,X_3>Y,X_4>Y,X_5>Y]\\
    &=1-P(X_1>Y)P(X_2>Y)P(X_3>Y)P(X_4>Y)P(X_5>Y)\\
    &=1-(1-P(X_1\leqslant Y))(1-P(X_2\leqslant Y))(1-P(X_3\leqslant Y))(1-P(X_4\leqslant Y))(1-P(X_5\leqslant Y))\\
    &=1-(1-F(Y))^5\\
    &=1-(1-\frac{y}{10})^5\\
    &g(Y_S)=\frac{d}{dy}1-(1-\frac{y}{10})^5\\
    &=-5(1-\frac{y}{10})^4\times(-\frac{1}{10})\\
    &=\frac{1}{2}(1-\frac{y}{10})^4\\
    &E[Y_S]=\int_{0}^{10}y\frac{1}{2}(1-\frac{y}{10})^4dy\\
    &=\frac{1}{2\times10^4}\int_{0}^{10}y(y-10)^4dy\\
    &u\coloneqq y-10\\
    &du=dy\\
    \Rightarrow&E[Y_S]=\frac{1}{2\times10^4}\int_{-10}^{0}(u^5+10u^4)du\\
    &=\frac{1}{2\times10^4}\frac{100000}{3}\\
    &=1.67\\
    &E[Y_L]-E[Y_S]=\frac{50}{6}-\frac{10}{6}=\frac{20}{3}\\
\end{align*}

~

\subsection*{c}

~

\begin{align*}
    &h(Y_M)=\frac{n!}{(i-1)!(n-i)!}[F(Y)]^{i-1}[1-F(Y)]^{n-i}f(Y)\\
    &=\frac{5!}{2!2!}(\frac{y}{10})^2(1-\frac{y}{10})^2\frac{1}{10}\\
    &=3(\frac{y}{10})^2(1-\frac{y}{10})^2\\
    &E[Y_M]=\int_{0}^{10}yh(Y_M)dy\\
    &=0.03\int_{0}^{10}y^3(1-\frac{y}{10})^2dy\\
    &=0.03\times\frac{500}{3}\\
    &=5\\
\end{align*}

~

\subsection*{d}

~

\begin{align*}
    &V[Y_L]=E[{Y_L}^2]-E[Y_L]^2\\
    &=\int_{0}^{10}y^2\frac{5y^4}{10^5}dy-(\frac{50}{6})^2\\
    &=\frac{5}{10^5}\int_{0}^{10}y^6dy-\frac{625}{9}\\
    &=\frac{500}{7}-\frac{625}{9}\\
    &=1.984\\
    &\sigma=\sqrt{V[Y_L]}=\sqrt{1.984}=1.409\\
\end{align*}

\newpage

\section*{Question 2}

~

\subsection*{a}

~

\begin{align*}
    &P(X\geqslant5)=1-P(X<5)\\
    &=1-P(X_1<5)P(X_2<5)P(X_3<5)\\
    &=1-(P(X_i<5))^3\\
    &=1-(\int_{1}^{5}f(x)dx)^3\\
    &=1-(\int_{1}^{5}\frac{3}{x^4}dx)^3\\
    &=1-(\left[-\frac{1}{x^3}\right]^5_1)^3\\
    &=1-(\frac{124}{125})^3\\
    &=0.238\\
\end{align*}

~

\subsection*{b}

~

\begin{align*}
    &F(x)=\int_{1}^{x}f(t)dt\\
    &=\int_{1}^{x}\frac{3}{t^4}dt\\
    &=\left[-t^{-3}\right]^x_1\\
    &=1-\frac{1}{x^3}\\
    &g(x_3)=\frac{3!}{2!0!}[F(x_3)]^2(\frac{3}{x^4})\\
    &=3(1-\frac{1}{x^3})^2(\frac{3}{x^4})\\
    &E[X_3]=\int_{1}^{\infty}xg(x_3)dx\\
    &=\int_{1}^{\infty}x3(1-\frac{1}{x^3})^2(\frac{3}{x^4})dx\\
    &=9\left[-\frac{1}{2x^2}-\frac{1}{8x^8}+\frac{2}{5x^5}\right]^\infty_1\\
    &=9(\frac{1}{2}+\frac{1}{8}+\frac{2}{5})\\
    &=\frac{81}{40}\\
    &=2.025
\end{align*}

\newpage

\section*{Question 3}

~

\subsection*{a}

~

\begin{align*}
    &\hat{\lambda}=\overline{x}=\frac{\sum f(x)}{\sum f}\\
    &\sum f(x)=37+2\times42+3\times30+4\times13+5\times7+6\times2+7\times1\\
    &=317\\
    &\sum f=18+37+42+30+13+7+2+1=150\\
    \Rightarrow&\hat{\lambda}=\frac{317}{150}\\
\end{align*}

~

\subsection*{b}

~

\begin{align*}
    &V(X)=\lambda\\
    &V(\overline{X})=\frac{\lambda}{n}\\
    \Rightarrow&\hat{\sigma}=\sqrt{\frac{\hat{\lambda}}{n}}\\
    &=\sqrt{\frac{\frac{317}{150}}{150}}\\
    &=0.1187\\
\end{align*}

\newpage

\section*{Question 4}

~

\subsection*{a}

~

\begin{align*}
    &E[\frac{X_1}{n_1}-\frac{X_2}{n_2}]=\frac{1}{n_1}E[X_1]-\frac{1}{n_2}E[X_2]\\
    &=\frac{1}{n_1}(n_1p_1)-frac{1}{n_2}(n_2p_2)\\
    &=p_1-p_2\\
\end{align*}

~

\subsection*{b}

~

\begin{align*}
    &\sigma=\sqrt{V[\frac{X_1}{n_1}-\frac{X_2}{n_2}]}\\
    &=\sqrt{\frac{1}{{n_1}^2}V(X_1)+\frac{1}{{n_2}^2}V(X_2)}\\
    &=\sqrt{\frac{1}{{n_1}^2}n_1p_1(1-p_1)+\frac{1}{{n_2}^2}n_2p_2(1-p_2)}\\
    &=\sqrt{\frac{p_1(1-p_1)}{n_1}+\frac{p_2(1-p_2)}{n_2}}\\
\end{align*}

~

\subsection*{c}

~

\begin{align*}
    &\hat{p_1}=\frac{x_1}{n_1}\\
    &\hat{p_2}=\frac{x_2}{n_2}\\
    &\hat{sigma}=\sqrt{\frac{\hat{p_1}(1-\hat{p_1})}{n_1}+\frac{\hat{p_2}(1-\hat{p_2})}{n_2}}\\
    &=\sqrt{\frac{\frac{x_1}{n_1}(1-\frac{x_1}{n_1})}{n_1}+\frac{\frac{x_2}{n_2}(1-\frac{x_2}{n_2})}{n_2}}\\
    &=\sqrt{\frac{\frac{x_1(n_1-x_1)}{{n_1}^2}}{n_1}+\frac{\frac{x_2(n_2-x_2)}{{n_2}^2}}{n_2}}\\
    &=\sqrt{\frac{x_1(n_1-x_1)}{{n_1}^3}+\frac{x_2(n_2-x_2)}{{n_2}^3}}\\
\end{align*}

~

\subsection*{d}

~

\begin{align*}
    &\hat{p_1}-\hat{p_2}=\frac{x_1}{n_1}-\frac{x_2}{n_2}\\
    &=\frac{127}{200}-\frac{176}{200}\\
    &=-\frac{49}{200}\\
\end{align*}

~

\subsection*{e}

~

\begin{align*}
    &\hat{\sigma}=\sqrt{\frac{x_1(n_1-x_1)}{{n_1}^3}+\frac{x_2(n_2-x_2)}{{n_2}^3}}\\
    &=\sqrt{\frac{127(200-127)}{200^3}+\frac{176(200-176)}{200^3}}\\
    &=0.0411\\
\end{align*}

\newpage

\section*{Question 5}

~

\subsection*{a}

~

\begin{align*}
    &E[X]=\int_{0}^{1}xf(x)dx\\
    &=\int_{0}^{1}x(\theta+1)x^\theta dx\\
    &=\int_{0}^{1}(\theta+1)x^{\theta+1}dx\\
    &=\left[\frac{\theta+1}{\theta+2}x^{\theta+2}\right]^1_0\\
    &=\frac{\theta+1}{\theta+2}\\
    \Rightarrow&\overline{X}=\frac{\theta+1}{\theta+2}\\
    &\theta\overline{X}+2\overline{X}=\theta+1\\
    &\theta=\frac{1-2\overline{X}}{\overline{X}-1}\\
    &\overline{X}=\frac{\sum x}{n}\\
    &=\frac{0.92+0.79+0.90+0.65+0.86+0.47+0.73+0.97+0.94+0.77}{10}\\
    &=0.8\\
    &\theta=\frac{1-2\times0.8}{0.8-1}=3\\
\end{align*}

~

\subsection*{b}

~

\begin{align*}
    &L=\prod_{i=1}^{10}(\theta+1)x_i^\theta\\
    &=(\theta+1)^10\prod_{i=1}^{10}x_i^\theta\\
    &\ln L=10\ln(\theta+1)+\theta\sum_{i=1}^{10}\ln x_i\\
    &\frac{d \ln L}{theta}=\frac{10}{\theta+1}+\sum_{i=1}^{10}\ln x_i=0\\
    &\frac{10}{\theta+1}=-\sum_{i=1}^{10}\ln x_i\\
    &\theta=-\frac{10}{\sum_{i=1}^{10}\ln x_i}-1\\
    &\sum_{i=1}^{10}\ln x_i=\ln0.92+\ln0.79+\ln0.90+\ln0.65\\
    &+\ln0.86+\ln0.47+\ln0.73+\ln0.97+\ln0.94+\ln0.77\\
    &=-2.4295\\
    &\theta=-\frac{10}{-2.4295}-1\\
    &=3.12\\
\end{align*}

\newpage

\section*{Collaborators}

~

Frank Zhu

~

Jeffery Shu

~

Sam Sun
\end{document}